theories/Views/PropD.v
@@ -1,8 +1,9 @@
+(*
 Require Import MirrorCore.Views.TrmD.
 
 Section PropD.
   Context {typ : Type} {RType_typ : RType typ}.
-  
+
   Context {Typ0_tyProp : Typ0 _ Prop}.
 
   Let tyProp : typ := @typ0 _ _ _ Typ0_tyProp.
@@ -14,3 +15,4 @@ Section PropD.
     trmD P (typ0_cast (Typ0 := Typ0_tyProp)).
 
 End PropD.
+*)
